Nun die andere Richtung der Aussage
\begin{align*}
    \forall y\forall x\varphi(x,y) \models\forall x\forall y\varphi(x, y)
\end{align*}
als Warheitsbaum.

\begin{figure}[h]
\centering
\begin{tikzpicture}
    \node (01) [a] {$\forall y\forall x\varphi(x, y)$ (01)};
    \node (02) [b, below of=01] {$\neg\forall x\forall y\varphi(x, y)$ (02)};
    \node (03) [b, below of=02] {$\exists x\exists y\neg\varphi(x, y)$ (03)};
    \node (04) [b, below of=03] {$\exists y\neg\varphi(a, y)$ (04)};
    \node (05) [b, below of=04] {$\neg\varphi(a, b)$ (05)};
    \node (06) [a, below of=05] {$\forall y\varphi(a, y)$ (06)};
    \node (07) [a, below of=06] {$\varphi(a, b)$ (07)};

    \node (08) [below of=07, yshift=3mm] {$(07)\lightning(05)$};

    \draw (01) -- (02) -- (03) -- (04) -- (05) -- (06) -- (07);
\end{tikzpicture}
\caption{Die eine Richtung der Ã„quivalenz}
\label{fig:allAllChanged02}
\end{figure}
